added Isabelle lemma that defines inverse in terms of SOME
git-svn-id: svn+ssh://svn.kestrel.edu/Specware/trunk@5381 7b97033b-253e-4a5c-9b07-e25f9089a9fd

Library/Isa/Function.thy
@@ -1,5 +1,5 @@
 theory Function
-imports IsabelleExtensions
+imports Boolean
 begin
 theorem Function__id__def: 
   "id x = x"
@@ -11,8 +11,8 @@ theorem Function__identity__stp:
   "\<lbrakk>Fun_PD P__a f\<rbrakk> \<Longrightarrow> 
    RFun P__a (id o f) = f 
      \<and> RFun P__a (f o id) = f"
-    apply(auto)
-    apply(rule ext, simp)+
+  apply(auto)
+  apply(rule ext, simp)+
   done
 theorem Function__identity: 
   "id o f = f \<and> f o id = f"
@@ -20,11 +20,11 @@ theorem Function__identity:
 theorem Function__associativity__stp: 
   "\<lbrakk>Fun_PD P__a f\<rbrakk> \<Longrightarrow> 
    RFun P__a ((h o g) o f) = RFun P__a (h o (g o f))"
-    apply(rule ext, simp)
+  apply(rule ext, simp)
   done
 theorem Function__associativity: 
   "(h o g) o f = h o (g o f)"
-    apply(simp add: o_assoc)
+  apply(simp add: o_assoc)
   done
 theorem Function__e_cl_gt__def: 
   "g o f = g o f"
@@ -38,168 +38,206 @@ defs Function__injective_p__stp_def:
 theorem Function__injective_p__def: 
   "inj f 
      = (\<forall>(x1::'a) (x2::'a). f x1 = f x2 \<longrightarrow> x1 = x2)"
-    apply(simp add: inj_on_def)
+  apply(simp add: inj_on_def)
   done
 
 lemma Function__injective_p__stp_simp [simp]:
   "Function__injective_p__stp P f = (inj_on f P)"
   by (auto simp add: Function__injective_p__stp_def inj_on_def mem_def)
-  
+
 consts Function__surjective_p__stp :: "('a \<Rightarrow> bool) \<times> ('b \<Rightarrow> bool) \<Rightarrow> 
                                        ('a \<Rightarrow> 'b) \<Rightarrow> bool"
 defs Function__surjective_p__stp_def: 
   "Function__surjective_p__stp
-     \<equiv> (\<lambda> ((P__a::'a \<Rightarrow> bool),(P__b::'b \<Rightarrow> bool)). 
+     \<equiv> (\<lambda> ((P__a::'a \<Rightarrow> bool), (P__b::'b \<Rightarrow> bool)). 
           \<lambda> (f::'a \<Rightarrow> 'b). 
             \<forall>(y::'b). 
               P__b y 
                 \<longrightarrow> (\<exists>(x::'a). P__a x \<and> f x = y))"
 theorem Function__surjective_p__def: 
   "surj f = (\<forall>(y::'b). \<exists>(x::'a). f x = y)"
-    apply(simp add: surj_def eq_commute)
+  apply(simp add: surj_def eq_commute)
   done
 
 lemma Function__surjective_p__stp_simp[simp]:
   "Function__surjective_p__stp (A,B) f = surj_on f A B"
-  by (auto simp add: Function__surjective_p__stp_def Ball_def Bex_def mem_def surj_on_def)
+  by (auto simp add: Function__surjective_p__stp_def
+                     Ball_def Bex_def mem_def surj_on_def)
 
 consts Function__bijective_p__stp :: "('a \<Rightarrow> bool) \<times> ('b \<Rightarrow> bool) \<Rightarrow> 
                                       ('a \<Rightarrow> 'b) \<Rightarrow> bool"
 defs Function__bijective_p__stp_def: 
   "Function__bijective_p__stp
-     \<equiv> (\<lambda> ((P__a::'a \<Rightarrow> bool),(P__b::'b \<Rightarrow> bool)). 
+     \<equiv> (\<lambda> ((P__a::'a \<Rightarrow> bool), (P__b::'b \<Rightarrow> bool)). 
           \<lambda> (f::'a \<Rightarrow> 'b). 
             Function__injective_p__stp P__a f 
-              \<and> Function__surjective_p__stp(P__a,P__b) f)"
+              \<and> Function__surjective_p__stp(P__a, P__b) f)"
 theorem Function__bijective_p__def: 
   "bij f = (inj f \<and> surj f)"
-    apply(simp add: bij_def)
+  apply(simp add: bij_def)
   done
 
-lemma Function__bijective_p__stp_simp[simp]:
-  "Function__bijective_p__stp (A,B) f = bij_ON f A B"
-  by (simp add: Function__bijective_p__stp_def bij_ON_def)
-lemma Function__bijective_p__stp_univ[simp]:
-  "Function__bijective_p__stp (A,\<lambda> x. True) f = bij_on f A UNIV"
-  by (simp add: univ_true bij_ON_UNIV_bij_on)
-
-lemma Function__bij_inv_stp:
-   "Function__bijective_p__stp (A,\<lambda> x. True) f \<Longrightarrow> Function__bijective_p__stp (\<lambda>x. True, A) (inv_on A f)"
-   by (simp add: univ_true bij_ON_imp_bij_ON_inv)
+  lemma Function__bijective_p__stp_simp[simp]:
+    "Function__bijective_p__stp (A,B) f = bij_ON f A B"
+    by (simp add: Function__bijective_p__stp_def bij_ON_def)
+  lemma Function__bijective_p__stp_univ[simp]:
+    "Function__bijective_p__stp (A,\<lambda> x. True) f = bij_on f A UNIV"
+    by (simp add: univ_true bij_ON_UNIV_bij_on)
+  lemma Function__bij_inv_stp:
+    "Function__bijective_p__stp (A,\<lambda> x. True) f \<Longrightarrow>
+     Function__bijective_p__stp (\<lambda>x. True, A) (inv_on A f)"
+    by (simp add: univ_true bij_ON_imp_bij_ON_inv)
 
 types  ('a,'b)Function__Injection = "'a \<Rightarrow> 'b"
 types  ('a,'b)Function__Surjection = "'a \<Rightarrow> 'b"
 types  ('a,'b)Function__Bijection = "'a \<Rightarrow> 'b"
 theorem Function__inverse__stp_Obligation_subtype: 
-  "\<lbrakk>Function__bijective_p__stp(P__a,\<lambda> ignore. True) f; 
+  "\<lbrakk>Function__bijective_p__stp(P__a, \<lambda> ignore. True) f; 
     Fun_PD P__a f; 
-    Function__bijective_p__stp(P__a,\<lambda> ignore. True) f\<rbrakk> \<Longrightarrow> 
-   Function__bijective_p__stp(\<lambda> ignore. True,P__a)
+    Function__bijective_p__stp(P__a, \<lambda> ignore. True) f\<rbrakk> \<Longrightarrow> 
+   Function__bijective_p__stp(\<lambda> ignore. True, P__a)
       (\<lambda> (y::'b). (THE (x::'a). P__a x \<and> f x = y))"
-    apply(simp only: Function__bijective_p__stp_simp univ_true)
-    apply(subgoal_tac "(\<lambda>y. THE x. P__a x \<and> f x = y) = inv_on P__a f", simp)
-    apply(simp add: bij_ON_imp_bij_ON_inv)
-    apply(auto simp add: bij_ON_def, 
-          thin_tac "\<forall>x0. \<not> P__a x0 \<longrightarrow> f x0 = regular_val")
-    apply(rule ext)
-    apply(rule the_equality, auto)
-    apply(simp add: surj_on_def Bex_def)
-    apply(drule_tac x="y" in spec, auto simp add: mem_def)
+  apply(simp only: Function__bijective_p__stp_simp univ_true)
+  apply(subgoal_tac "(\<lambda>y. THE x. P__a x \<and> f x = y) = inv_on P__a f",
+        simp)
+  apply(simp add: bij_ON_imp_bij_ON_inv)
+  apply(auto simp add: bij_ON_def, 
+        thin_tac
+          "\<forall>x0. \<not> P__a x0 \<longrightarrow> f x0 = regular_val")
+  apply(rule ext)
+  apply(rule the_equality, auto)
+  apply(simp add: surj_on_def Bex_def)
+  apply(drule_tac x="y" in spec, auto simp add: mem_def)
   done
 theorem Function__inverse__stp_Obligation_the: 
-  "\<lbrakk>Function__bijective_p__stp((P__a::'a \<Rightarrow> bool),\<lambda> ignore. True) (f::'a \<Rightarrow> 'b); 
+  "\<lbrakk>Function__bijective_p__stp((P__a::'a \<Rightarrow> bool), \<lambda> ignore. True) (f::'a \<Rightarrow> 'b); 
     Fun_PD P__a f; 
     P__a (x::'a); 
-    Function__bijective_p__stp(P__a,\<lambda> ignore. True) f; 
+    Function__bijective_p__stp(P__a, \<lambda> ignore. True) f; 
     P__a x\<rbrakk> \<Longrightarrow> \<exists>!(x::'a). P__a x \<and> f x = (y::'b)"
-    apply(auto simp add: bij_ON_def surj_on_def Ball_def Bex_def inj_on_def mem_def)
-    apply(rotate_tac -1, drule_tac x="y" in spec, auto)
+  apply(auto simp add:
+          bij_ON_def surj_on_def Ball_def Bex_def inj_on_def mem_def)
+  apply(rotate_tac -1, drule_tac x="y" in spec, auto)
   done
 consts Function__inverse__stp :: "('a \<Rightarrow> bool) \<Rightarrow> ('a \<Rightarrow> 'b) \<Rightarrow> 'b \<Rightarrow> 'a"
 defs Function__inverse__stp_def: 
-  "Function__inverse__stp P__a f y
-     \<equiv> (THE (x::'a). P__a x \<and> f x = y)"
+  "Function__inverse__stp P__a f
+     \<equiv> (\<lambda> (y::'b). (THE (x::'a). P__a x \<and> f x = y))"
 theorem Function__inverse_Obligation_subtype: 
   "\<lbrakk>bij f\<rbrakk> \<Longrightarrow> 
    bij
-      (\<lambda> (y::'b). (THE (x::'a). (f:: ('a,'b)Function__Bijection) x = y))"
-    apply(subgoal_tac "( \<lambda>y. THE x. f x = y) = inv f")
-    apply(auto simp add: bij_def)
-    apply(erule surj_imp_inj_inv)
-    apply(erule inj_imp_surj_inv)
-    apply(rule ext, rule the_equality, auto simp add: surj_f_inv_f)
+      (\<lambda> (y::'b). (THE (x::'a). (f:: ('a, 'b)Function__Bijection) x = y))"
+  apply(subgoal_tac "( \<lambda>y. THE x. f x = y) = inv f")
+  apply(auto simp add: bij_def)
+  apply(erule surj_imp_inj_inv)
+  apply(erule inj_imp_surj_inv)
+  apply(rule ext, rule the_equality, auto simp add: surj_f_inv_f)
   done
 theorem Function__inverse_Obligation_the: 
   "\<lbrakk>bij f\<rbrakk> \<Longrightarrow> 
-   \<exists>!(x::'a). (f:: ('a,'b)Function__Bijection) x = (y::'b)"
-    apply(auto simp add: bij_def surj_def inj_on_def)
-    apply(drule spec, erule exE, drule sym, auto)
+   \<exists>!(x::'a). (f:: ('a, 'b)Function__Bijection) x = (y::'b)"
+  apply(auto simp add: bij_def surj_def inj_on_def)
+  apply(drule spec, erule exE, drule sym, auto)
   done
 theorem Function__inverse_subtype_constr: 
   "\<lbrakk>bij dom_inverse\<rbrakk> \<Longrightarrow> bij (inv dom_inverse)"
-    apply(auto simp add: bij_def)
-    apply(erule surj_imp_inj_inv)
-    apply(erule inj_imp_surj_inv)
+  apply(auto simp add: bij_def)
+  apply(erule surj_imp_inj_inv)
+  apply(erule inj_imp_surj_inv)
   done
 theorem Function__inverse__def: 
   "\<lbrakk>bij f\<rbrakk> \<Longrightarrow> inv f y = (THE (x::'a). f x = y)"
-    apply(rule sym, rule the_equality)
-    apply(auto simp add: bij_def surj_f_inv_f)
+  apply(rule sym, rule the_equality)
+  apply(auto simp add: bij_def surj_f_inv_f)
   done
 
-lemma Function__inverse__stp_alt:
-   "\<lbrakk>inj_on f A; y \<in> f`A\<rbrakk> \<Longrightarrow> Function__inverse__stp A f y = inv_on A f y"
-   by (auto simp add: Function__inverse__stp_def, 
-       rule the_equality, auto simp add:mem_def inj_on_def)
-
-lemma Function__inverse__stp_apply [simp]:
-   "\<lbrakk>bij_ON f A B; y \<in> B\<rbrakk> \<Longrightarrow> Function__inverse__stp A f y = inv_on A f y"
+  lemma Function__inverse__stp_alt:
+    "\<lbrakk>inj_on f A; y \<in> f`A\<rbrakk> \<Longrightarrow>
+     Function__inverse__stp A f y = inv_on A f y"
+    by (auto simp add: Function__inverse__stp_def, 
+        rule the_equality, auto simp add:mem_def inj_on_def)
+  lemma Function__inverse__stp_apply [simp]:
+    "\<lbrakk>bij_ON f A B; y \<in> B\<rbrakk> \<Longrightarrow>
+     Function__inverse__stp A f y = inv_on A f y"
     by(auto simp add: bij_ON_def surj_on_def,
        erule Function__inverse__stp_alt,
        simp add: image_def)
+  lemma Function__inverse__stp_simp:
+    "bij_on f A UNIV \<Longrightarrow> Function__inverse__stp A f = inv_on A f"
+    by (rule ext, simp add: bij_ON_UNIV_bij_on [symmetric])
 
-lemma Function__inverse__stp_simp:
-   "bij_on f A UNIV \<Longrightarrow> Function__inverse__stp A f = inv_on A f"
-   by (rule ext, simp add: bij_ON_UNIV_bij_on [symmetric])
+
+lemma inverse_SOME:
+ "\<lbrakk> Function__bijective_p__stp (domP,codP) f ; codP y \<rbrakk>
+  \<Longrightarrow>
+  Function__inverse__stp domP f y = (SOME x. domP x \<and> f x = y)"
+proof (auto simp add: Function__bijective_p__stp_def Function__inverse__stp_def)
+ assume CY: "codP y"
+ assume INJ: "inj_on f domP"
+ assume SURJ: "surj_on f domP codP"
+ from SURJ have "\<forall>y \<in> codP. \<exists>x \<in> domP. f x = y"
+  by (auto simp add: surj_on_def)
+ with CY have "\<exists>x \<in> domP. f x = y" by (auto simp add: mem_def)
+ then obtain x where DX: "domP x" and YX: "f x = y"
+  by (auto simp add: mem_def)
+ hence X: "domP x \<and> f x = y" by auto
+ have "\<And>x'. domP x' \<and> f x' = y \<Longrightarrow> x' = x"
+ proof -
+  fix x'
+  assume "domP x' \<and> f x' = y"
+  hence DX': "domP x'" and YX': "f x' = y" by auto
+  from INJ have
+   "\<forall>x \<in> domP. \<forall>x' \<in> domP.
+      f x = f x' \<longrightarrow> x = x'"
+   by (auto simp add: inj_on_def)
+  with DX DX' have "f x = f x' \<Longrightarrow> x = x'"
+   by (auto simp add: mem_def)
+  with YX YX' show "x' = x" by auto
+ qed
+ with X have "\<exists>!x. domP x \<and> f x = y" by (auto simp add: mem_def)
+ thus "(THE x. domP x \<and> f x = y) = (SOME x. domP x \<and> f x = y)"
+  by (rule THE_SOME)
+qed
 
 theorem Function__inverse_comp__stp [simp]: 
-  "\<lbrakk>Function__bijective_p__stp(P__a,P__b) f; Fun_P(P__a,P__b) f\<rbrakk> \<Longrightarrow> 
+  "\<lbrakk>Function__bijective_p__stp(P__a, P__b) f; 
+    Fun_P(P__a, P__b) f\<rbrakk> \<Longrightarrow> 
    RFun P__b (f o Function__inverse__stp P__a f) 
      = RFun P__b id 
      \<and> RFun P__a (Function__inverse__stp P__a f o f) 
          = RFun P__a id"
-    apply(auto)
-    apply(rule ext, clarsimp simp add: mem_def bij_ON_def)
-    apply(rule ext, clarsimp simp add: mem_def bij_ON_def)
+  apply(auto)
+  apply(rule ext, clarsimp simp add: mem_def bij_ON_def)
+  apply(rule ext, clarsimp simp add: mem_def bij_ON_def)
   done
 theorem Function__inverse_comp: 
   "\<lbrakk>bij f\<rbrakk> \<Longrightarrow> f o inv f = id \<and> inv f o f = id"
-    apply(simp add: bij_def surj_iff inj_iff)
+  apply(simp add: bij_def surj_iff inj_iff)
   done
 theorem Function__f_inverse_apply__stp: 
-  "\<lbrakk>Function__bijective_p__stp(P__a,(P__b::'b \<Rightarrow> bool)) f; 
-    Fun_P(P__a,P__b) f; 
+  "\<lbrakk>Function__bijective_p__stp(P__a, (P__b::'b \<Rightarrow> bool)) f; 
+    Fun_P(P__a, P__b) f; 
     P__b x\<rbrakk> \<Longrightarrow> f (Function__inverse__stp P__a f x) = x"
-    apply(auto simp add: mem_def bij_ON_def)
+  apply(auto simp add: mem_def bij_ON_def)
   done
 theorem Function__f_inverse_apply: 
   "\<lbrakk>bij f\<rbrakk> \<Longrightarrow> f (inv f x) = x"
-    apply(simp add: bij_def surj_f_inv_f)
+  apply(simp add: bij_def surj_f_inv_f)
   done
 theorem Function__inverse_f_apply__stp: 
-  "\<lbrakk>Function__bijective_p__stp(P__a,\<lambda> ignore. True) f; 
+  "\<lbrakk>Function__bijective_p__stp(P__a, \<lambda> ignore. True) f; 
     Fun_PD P__a f; 
     P__a (x::'a)\<rbrakk> \<Longrightarrow> 
    Function__inverse__stp P__a f (f x) = x"
-    apply(auto simp add: mem_def bij_ON_def)
+  apply(auto simp add: mem_def bij_ON_def)
   done
 theorem Function__inverse_f_apply: 
   "\<lbrakk>bij f\<rbrakk> \<Longrightarrow> inv f (f (x::'a)) = x"
-    apply(simp add: bij_def inv_f_f)
+  apply(simp add: bij_def inv_f_f)
   done
 theorem Function__eta__stp: 
   "\<lbrakk>Fun_PD P__a f\<rbrakk> \<Longrightarrow> RFun P__a (\<lambda> (x::'a). f x) = f"
-    apply(rule ext, simp)
+  apply(rule ext, simp)
   done
 theorem Function__eta: 
   "(\<lambda> (x::'a). (f::'a \<Rightarrow> 'b) x) = f"
@@ -215,7 +253,7 @@ defs Function__wellFounded_p__stp_def:
                       P__a y 
                         \<and> (p y 
                          \<and> (\<forall>(x::'a). 
-                              P__a x \<longrightarrow> (p x \<longrightarrow> \<not> (rel(x,y))))))))"
+                              P__a x \<longrightarrow> (p x \<longrightarrow> \<not> (rel(x, y))))))))"
 consts Function__wellFounded_p :: "('a \<times> 'a \<Rightarrow> bool) \<Rightarrow> bool"
 defs Function__wellFounded_p_def: 
   "Function__wellFounded_p rel
@@ -223,7 +261,7 @@ defs Function__wellFounded_p_def:
           (\<exists>(y::'a). p y) 
             \<longrightarrow> (\<exists>(y::'a). 
                    p y 
-                     \<and> (\<forall>(x::'a). p x \<longrightarrow> \<not> (rel(x,y)))))"
+                     \<and> (\<forall>(x::'a). p x \<longrightarrow> \<not> (rel(x, y)))))"
 consts Function__wfo__stp :: "('a \<Rightarrow> bool) \<Rightarrow> ('a \<times> 'a \<Rightarrow> bool) \<Rightarrow> bool"
 defs Function__wfo__stp_def: 
   "Function__wfo__stp P__a \<equiv> Function__wellFounded_p__stp P__a"
